simplify the proof.

core.v
@@ -3,45 +3,9 @@ Require Import Arith.
 Require Import List.
 Require Import Omega.
 
-Inductive term : Set :=
-  | term_pop  : term
-  | term_dup  : term
-  | term_swap : term
-  | term_push : term -> term
-  | term_seq  : term -> term -> term
-  | term_exec : term.
+Notation "[]" := nil : list_scope.
 
-Definition stack : Set := list term.
-
-(* Environment is product of the value stack and the continuacion stack. *)
-Definition environment : Set := (stack * stack)%type.
-
-Inductive reduction : relation environment :=
-  | red_pop  : forall (v : term) (vs ps : stack),
-               reduction ((v :: vs), (term_pop :: ps)) (vs, ps)
-  | red_dup  : forall (v : term) (vs ps : stack),
-               reduction ((v :: vs), (term_dup :: ps)) ((v :: v :: vs), ps)
-  | red_swap : forall (v1 v2 : term) (vs ps : stack),
-               reduction ((v1 :: v2 :: vs), (term_swap :: ps)) ((v2 :: v1 :: vs), ps)
-  | red_push : forall (v : term) (vs ps : stack),
-               reduction (vs, (term_push v :: ps)) ((v :: vs) , ps)
-  | red_seq  : forall (p1 p2 : term) (vs ps : stack),
-               reduction (vs, (term_seq p1 p2 :: ps)) (vs, (p1 :: p2 :: ps))
-  | red_exec : forall (p : term) (vs ps : stack),
-               reduction ((p :: vs), (term_exec :: ps)) (vs, (p :: ps)).
-
-Definition redstar : relation environment := clos_refl_trans _ reduction.
-
-Definition termnop : term := term_seq (term_push term_pop) term_pop.
-
-Lemma termnop_proof : forall (vs ps : stack),
-  redstar (vs, (termnop :: ps)) (vs, ps).
-  intros.
-  unfold termnop.
-  apply (rt_trans _ _ _ _ _ (rt_step _ _ _ _ (red_seq _ _ _ _))).
-  apply (rt_trans _ _ _ _ _ (rt_step _ _ _ _ (red_push _ _ _))).
-  apply (rt_step _ _ _ _ (red_pop _ _ _)).
-Qed.
+Notation "[ a ; .. ; b ]" := (a :: .. (b :: []) ..) : list_scope.
 
 Fixpoint replicate {A : Set} (n : nat) (a : A) :=
   match n with
@@ -53,37 +17,158 @@ Lemma app_replicate : forall (A : Set) (n m : nat) (a : A),
   replicate n a ++ replicate m a = replicate (n + m) a.
   intros.
   induction n.
-  unfold replicate, app ; auto.
-  assert (S n + m = S (n + m)).
-  omega.
-  rewrite H.
-  unfold replicate, app ; f_equal ; apply IHn.
+  compute ; auto.
+  replace (S n + m) with (S (n + m)) by omega.
+  compute ; f_equal ; apply IHn.
+Qed.
+
+Inductive term : Set :=
+  (* value stack operators *)
+  | term_pop  : term
+  | term_dup  : term
+  | term_swap : term
+  | term_cons : term
+  (* continuation stack operators *)
+  | term_push : term
+  | term_exec : term
+  (* structure *)
+  | term_seq  : term -> term -> term.
+
+Definition stack : Set := list term.
+
+(* Environment is product of the value stack and the continuacion stack. *)
+Definition environment : Set := (stack * stack)%type.
+
+Inductive reduction : relation environment :=
+  | reduction_pop  : forall (v : term) (vs ps : stack),
+                     reduction (v :: vs, term_pop :: ps) (vs, ps)
+  | reduction_dup  : forall (v : term) (vs ps : stack),
+                     reduction (v :: vs, term_dup :: ps) (v :: v :: vs, ps)
+  | reduction_swap : forall (v1 v2 : term) (vs ps : stack),
+                     reduction (v1 :: v2 :: vs, term_swap :: ps) (v2 :: v1 :: vs, ps)
+  | reduction_cons : forall (v1 v2 : term) (vs ps : stack),
+                     reduction (v1 :: v2 :: vs, term_cons :: ps) (term_seq v1 v2 :: vs, ps)
+  | reduction_push : forall (v : term) (vs ps : stack),
+                     reduction (vs, term_push :: v :: ps) (v :: vs, ps)
+  | reduction_exec : forall (p : term) (vs ps : stack),
+                     reduction (p :: vs, term_exec :: ps) (vs, p :: ps)
+  | reduction_seq  : forall (p1 p2 : term) (vs ps : stack),
+                     reduction (vs, term_seq p1 p2 :: ps) (vs, p1 :: p2 :: ps).
+
+Definition redstar : relation environment := clos_refl_trans _ reduction.
+
+Lemma decide_reduction : forall (e1 : environment),
+  (exists e2 : environment, reduction e1 e2) \/
+  ~(exists e2 : environment, reduction e1 e2).
+  intros.
+  destruct e1.
+  destruct s0.
+  right ; intro.
+  destruct H.
+  inversion H.
+  destruct t.
+  destruct s.
+  right ; intro ; destruct H ; inversion H.
+  left ; eexists ; apply reduction_pop.
+  destruct s.
+  right ; intro ; destruct H ; inversion H.
+  left ; eexists ; apply reduction_dup.
+  destruct s.
+  right ; intro ; destruct H ; inversion H.
+  destruct s.
+  right ; intro ; destruct H ; inversion H.
+  left ; eexists ; apply reduction_swap.
+  destruct s.
+  right ; intro ; destruct H ; inversion H.
+  destruct s.
+  right ; intro ; destruct H ; inversion H.
+  left ; eexists ; apply reduction_cons.
+  destruct s0.
+  right ; intro ; destruct H ; inversion H.
+  left ; eexists ; apply reduction_push.
+  destruct s.
+  right ; intro ; destruct H ; inversion H.
+  left ; eexists ; apply reduction_exec.
+  left ; eexists ; apply reduction_seq.
+Defined.
+
+Lemma reduction_unique : forall (a b c : environment),
+  reduction a b -> reduction a c -> b = c.
+  intros.
+  destruct a, b, c.
+  destruct s0.
+  inversion H.
+  destruct t.
+  destruct s ; [ inversion H | inversion H ; inversion H0 ; congruence ].
+  destruct s ; [ inversion H | inversion H ; inversion H0 ; congruence ].
+  destruct s ; [ inversion H | inversion H ; inversion H0 ; congruence ].
+  destruct s ; [ inversion H | inversion H ; inversion H0 ; congruence ].
+  destruct s ; [ inversion H | inversion H ; inversion H0 ; congruence ].
+  destruct s0 ; [ inversion H | inversion H ; inversion H0 ; congruence ].
+  destruct s ; [ inversion H | inversion H ; inversion H0 ; congruence ].
+  inversion H ; inversion H0 ; congruence.
+Qed.
+
+Ltac evalstep' e1 e2 :=
+  try apply rt_refl ;
+  lazymatch eval compute in (decide_reduction e1) with
+    | or_introl _ (ex_intro _ ?e3 ?p) =>
+      apply (rt_step _ _ _ _ p) ||
+      apply (rt_trans _ _ _ _ _ (rt_step _ _ _ _ p))
+    | or_intror _ _ => idtac
+    | _ => idtac
+  end.
+
+Ltac evalstep :=
+  match goal with
+    | |- redstar ?e1 ?e2 => evalstep' e1 e2
+    | |- clos_refl_trans _ reduction ?e1 ?e2 => evalstep' e1 e2
+    | _ => idtac
+  end.
+
+Definition termnop : term := term_seq (term_seq term_push term_pop) term_pop.
+
+Lemma rednop : forall (vs ps : stack), redstar (vs, termnop :: ps) (vs, ps).
+  intros ; repeat evalstep.
+Qed.
+
+Definition term_list (ts : list term) : term := fold_left term_seq ts termnop.
+
+Lemma term_list_prop : forall (ts : list term) (vs ps : stack),
+  redstar (vs, term_list ts :: ps) (vs, ts ++ ps).
+  intros ; compute.
+  assert (forall head, redstar (vs, fold_left term_seq ts head :: ps) (vs, head :: ts ++ ps)).
+    induction ts ; intros.
+    evalstep.
+    apply (rt_trans _ _ _ _ _ (IHts (term_seq head a))) ; evalstep.
+  apply (rt_trans _ _ _ _ _ (H termnop) (rednop _ _)).
+Qed.
+
+Definition term_quote : term := term_list [term_push ; term_push ; term_cons].
+
+Lemma term_quote_prop : forall (v : term) (vs ps : stack),
+  redstar (v :: vs, term_quote :: ps) (term_seq term_push v :: vs, ps).
+  intros ; repeat evalstep.
 Qed.
 
 Definition termnat (n : nat) (p : term) : Set :=
   forall (v : term) (vs ps : stack),
-    redstar ((v :: vs), (p :: ps)) (replicate (S n) v ++ vs, ps).
+    redstar (v :: vs, p :: ps) (vs, replicate n v ++ ps).
 
-Fixpoint termnat_term (n : nat) : term :=
-  match n with
-    | 0 => termnop
-    | S n => term_seq term_dup (termnat_term n)
-  end.
+Definition termnat_term_part : term := term_list [
+  term_dup ; term_quote ; term_swap ; term_quote ; term_cons ;
+  term_swap ; term_quote ; term_swap ; term_cons ; term_exec ;
+  term_swap ; term_cons ; term_swap ].
 
-Lemma termnat_proof : forall (n : nat), termnat n (termnat_term n).
-  intros.
-  induction n ; unfold termnat ; intros.
-  apply termnop_proof.
-  apply (rt_trans _ _ _ _ _ (rt_step _ _ _ _ (red_seq _ _ _ _))).
-  apply (rt_trans _ _ _ _ _ (rt_step _ _ _ _ (red_dup _ _ _))).
-  assert (replicate (S (S n)) v = replicate (S n) v ++ replicate 1 v).
-    assert (S (S n) = S n + 1).
-      omega.
-    rewrite H.
-    apply eq_sym.
-    apply app_replicate.
-  rewrite H.
-  rewrite (eq_sym (app_assoc (replicate (S n) v) (replicate 1 v) vs)).
-  apply IHn.
+Lemma termnat_term_part_prop : forall (p1 p2 : term) (vs ps : stack),
+  redstar (p1 :: p2 :: vs, termnat_term_part :: ps) (p1 :: term_seq p1 p2 :: vs, ps).
+  intros ; repeat evalstep.
 Qed.
 
+Definition termnat_term (n : nat) : term := term_list
+  [ term_push ; termnop ; term_swap ;
+    term_list (replicate n termnat_term_part) ; term_pop ; term_exec ].
+
+Lemma termnat_prop : forall (n : nat), termnat n (termnat_term n).
+  repeat intro.
+  apply (rt_trans _ _ _ _ _ (term_list_prop _ _ _)).
